Refactored unitality and invertibility.

fowl/Is/Invertible.v
@@ -3,28 +3,146 @@
 From DEZ Require Export
   Init.
 
-(** ** Left Inverse of a Binary Function *)
+(** ** Left Invertible Binary Function *)
 
-Class IsInvL (A B C D : Type) (X : D -> B -> Prop)
-  (x : B) (f : A -> C) (k : C -> A -> D) : Prop :=
-  inv_l (y : A) : X (k (f y) y) x.
+Class IsInvBinFnL (A B C : Type) (X : C -> C -> Prop)
+  (x : C) (f : A -> B) (k : B -> A -> C) : Prop :=
+  inv_bin_fn_l (y : A) : X (k (f y) y) x.
 
-(** ** Right Inverse of a Binary Function *)
+(** ** Right Invertible Binary Function *)
 
-Class IsInvR (A B C D : Type) (X : D -> B -> Prop)
-  (x : B) (f : A -> C) (k : A -> C -> D) : Prop :=
-  inv_r (y : A) : X (k y (f y)) x.
+Class IsInvBinFnR (A B C : Type) (X : C -> C -> Prop)
+  (x : C) (f : A -> B) (k : A -> B -> C) : Prop :=
+  inv_bin_fn_r (y : A) : X (k y (f y)) x.
 
-(** ** Inverse of a Torsion *)
+(** ** Left Invertible Form *)
 
-Class IsInvLR2 (A B C : Type) (X : B -> B -> Prop)
-  (x : B) (f : A -> C) (k : C -> A -> B) (m : A -> C -> B) : Prop := {
-  is_inv_l :> IsInvL X x f k;
-  is_inv_r :> IsInvR X x f m;
+Class IsInvFormL (A B : Type) (X : B -> B -> Prop)
+  (x : B) (f : A -> A) (a : A -> A -> B) : Prop :=
+  inv_form_l (y : A) : X (a (f y) y) x.
+
+(** ** Right Invertible Form *)
+
+Class IsInvFormR (A B : Type) (X : B -> B -> Prop)
+  (x : B) (f : A -> A) (a : A -> A -> B) : Prop :=
+  inv_form_r (y : A) : X (a y (f y)) x.
+
+(** ** Invertible Form *)
+
+Class IsInvForm (A B : Type) (X : B -> B -> Prop)
+  (x : B) (f : A -> A) (a : A -> A -> B) : Prop := {
+  inv_form_is_inv_form_l :> IsInvFormL X x f a;
+  inv_form_is_inv_form_r :> IsInvFormR X x f a;
 }.
 
-(** ** Inverse of a Binary Operation *)
+Section Context.
 
-Class IsInvLR (A : Type) (X : A -> A -> Prop)
+Context (A : Type) (X : A -> A -> Prop)
+  (x : A) (f : A -> A) (a : A -> A -> A).
+
+(** Left invertible binary function implies left invertible form. *)
+
+#[export] Instance inv_bin_fn_l_is_inv_form_l
+  `{!IsInvBinFnL X x f a} : IsInvFormL X x f a.
+Proof. auto. Qed.
+
+(** Left invertible form implies left invertible binary function. *)
+
+#[local] Instance inv_form_l_is_inv_bin_fn_l
+  `{!IsInvFormL X x f a} : IsInvBinFnL X x f a.
+Proof. auto. Qed.
+
+(** Right invertible binary function implies right invertible form. *)
+
+#[export] Instance inv_bin_fn_r_is_inv_form_r
+  `{!IsInvBinFnR X x f a} : IsInvFormR X x f a.
+Proof. auto. Qed.
+
+(** Right invertible form implies right invertible binary function. *)
+
+#[local] Instance inv_form_r_is_inv_bin_fn_r
+  `{!IsInvFormR X x f a} : IsInvBinFnR X x f a.
+Proof. auto. Qed.
+
+End Context.
+
+(** ** Left Invertible Binary Operation *)
+
+(** This has the same shape as [Z.add_opp_diag_l]. *)
+
+Class IsInvL (A : Type) (X : A -> A -> Prop)
   (x : A) (f : A -> A) (k : A -> A -> A) : Prop :=
-  is_inv_l_r_2 :> IsInvLR2 X x f k k.
+  inv_l (y : A) : X (k (f y) y) x.
+
+(** ** Right Invertible Binary Operation *)
+
+(** This has the same shape as [Z.add_opp_diag_r]. *)
+
+Class IsInvR (A : Type) (X : A -> A -> Prop)
+  (x : A) (f : A -> A) (k : A -> A -> A) : Prop :=
+  inv_r (y : A) : X (k y (f y)) x.
+
+(** ** Invertible Binary Operation *)
+
+Class IsInv (A : Type) (X : A -> A -> Prop)
+  (x : A) (f : A -> A) (k : A -> A -> A) : Prop := {
+  inv_is_inv_l :> IsInvL X x f k;
+  inv_is_inv_r :> IsInvR X x f k;
+}.
+
+Section Context.
+
+Context (A : Type) (X : A -> A -> Prop)
+  (x : A) (f : A -> A) (k : A -> A -> A).
+
+(** Left invertible form implies left invertible binary operation. *)
+
+(** We cannot declare these definitions to be instances
+    until the end of this section if we want to avoid cycles. *)
+
+Lemma inv_form_l_is_inv_l
+  `{!IsInvFormL X x f k} : IsInvL X x f k.
+Proof. auto. Qed.
+
+(** Left invertible binary operation implies left invertible form. *)
+
+Lemma inv_l_is_inv_form_l
+  `{!IsInvL X x f k} : IsInvFormL X x f k.
+Proof. auto. Qed.
+
+(** Right invertible form implies right invertible binary operation. *)
+
+Lemma inv_form_r_is_inv_r
+  `{!IsInvFormR X x f k} : IsInvR X x f k.
+Proof. auto. Qed.
+
+(** Right invertible binary operation implies right invertible form. *)
+
+Lemma inv_r_is_inv_form_r
+  `{!IsInvR X x f k} : IsInvFormR X x f k.
+Proof. auto. Qed.
+
+(** Invertible binary function implies invertible form. *)
+
+#[export] Instance inv_form_is_inv
+  `{!IsInvForm X x f k} : IsInv X x f k.
+Proof.
+  esplit; eauto
+  using inv_form_l_is_inv_l, inv_form_r_is_inv_r
+  with typeclass_instances. Qed.
+
+(** Invertible form implies invertible binary function. *)
+
+#[local] Instance inv_is_inv_form
+  `{!IsInv X x f k} : IsInvForm X x f k.
+Proof.
+  esplit; eauto
+  using inv_l_is_inv_form_l, inv_r_is_inv_form_r
+  with typeclass_instances. Qed.
+
+#[export] Existing Instance inv_form_l_is_inv_l.
+#[local] Existing Instance inv_l_is_inv_form_l.
+#[export] Existing Instance inv_form_r_is_inv_r.
+#[local] Existing Instance inv_r_is_inv_form_r.
+
+End Context.
