fowl/Is/Group.v
@@ -6,22 +6,21 @@ From DEZ.Is Require Export
   Monoid Invertible Proper
   Fixed Involutive Injective Cancellative Distributive Preserving.
 From DEZ.Supports Require Import
-  EquivalenceNotations AdditiveNotations.
+  AdditiveNotations EquivalenceNotations.
 
 (** ** Group *)
 
 Class IsGrp (A : Type) (X : A -> A -> Prop)
   (x : A) (f : A -> A) (k : A -> A -> A) : Prop := {
-  is_mon :> IsMon X x k;
-  is_inv_l_r :> IsInvLR X x f k;
-  is_proper :> IsProper (X ==> X) f;
+  grp_is_mon :> IsMon X x k;
+  grp_is_inv :> IsInv X x f k;
+  grp_is_proper :> IsProper (X ==> X) f;
 }.
 
 Section Context.
 
 Context (A : Type) (X : A -> A -> Prop)
-  (x : A) (f : A -> A) (k : A -> A -> A)
-  `{!IsGrp X x f k}.
+  (x : A) (f : A -> A) (k : A -> A -> A) `{!IsGrp X x f k}.
 
 #[local] Instance has_equiv_rel : HasEquivRel A := X.
 #[local] Instance has_null_op : HasNullOp A := x.
@@ -34,18 +33,16 @@ Ltac note := progress (
   try change f with (un_op (A := A)) in *;
   try change k with (bin_op (A := A)) in *).
 
-#[local] Instance is_fixed : IsFixed X x f.
+#[export] Instance grp_is_fixed : IsFixed X x f.
 Proof.
-  note.
-  unfold IsFixed, IsFixed2.
+  note. unfold IsFixed, IsFixed2.
   setoid_rewrite <- (unl_r (- x)).
   setoid_rewrite (inv_l x).
   reflexivity. Qed.
 
-#[local] Instance is_invol : IsInvol X f.
+#[export] Instance grp_is_invol : IsInvol X f.
 Proof.
-  note.
-  intros y.
+  note. intros y.
   setoid_rewrite <- (unl_r (- (- y))).
   setoid_rewrite <- (inv_l y).
   setoid_rewrite (assoc (- (- y)) (- y) y).
@@ -53,10 +50,9 @@ Proof.
   setoid_rewrite (unl_l y).
   reflexivity. Qed.
 
-#[local] Instance is_inj : IsInj X f.
+#[export] Instance grp_is_inj : IsInj X f.
 Proof.
-  note.
-  intros y z a.
+  note. intros y z a.
   setoid_rewrite <- (unl_l z).
   setoid_rewrite <- (inv_r y).
   setoid_rewrite a.
@@ -65,10 +61,9 @@ Proof.
   setoid_rewrite (unl_r y).
   reflexivity. Qed.
 
-#[local] Instance is_cancel_l : IsCancelL X k.
+#[export] Instance grp_is_cancel_l : IsCancelL X k.
 Proof.
-  note.
-  intros y z w a.
+  note. intros y z w a.
   setoid_rewrite <- (unl_l y).
   setoid_rewrite <- (inv_l w).
   setoid_rewrite <- (assoc (- w) w y).
@@ -78,10 +73,9 @@ Proof.
   setoid_rewrite (unl_l z).
   reflexivity. Qed.
 
-#[local] Instance is_cancel_r : IsCancelR X k.
+#[export] Instance grp_is_cancel_r : IsCancelR X k.
 Proof.
-  note.
-  intros y z w a.
+  note. intros y z w a.
   setoid_rewrite <- (unl_r y).
   setoid_rewrite <- (inv_r w).
   setoid_rewrite (assoc y w (- w)).
@@ -91,13 +85,12 @@ Proof.
   setoid_rewrite (unl_r z).
   reflexivity. Qed.
 
-#[local] Instance is_cancel_l_r : IsCancelLR X k.
+#[export] Instance grp_is_cancel : IsCancel X k.
 Proof. esplit; typeclasses eauto. Qed.
 
-#[local] Instance is_antidistr : IsAntidistr X f k k.
+#[export] Instance grp_is_antidistr : IsAntidistr X f k k.
 Proof.
-  note.
-  intros y z.
+  note. intros y z.
   apply (cancel_l (- (y + z)) ((- z) + (- y)) (y + z)).
   setoid_rewrite (inv_r (y + z)).
   setoid_rewrite (assoc (y + z) (- z) (- y)).
@@ -108,9 +101,6 @@ Proof.
   reflexivity. Qed.
 
 End Context.
-
-#[export] Hint Resolve is_fixed is_invol is_inj
-  is_cancel_l is_cancel_r is_cancel_l_r is_antidistr : typeclass_instances.
 
 From Coq Require Import
   ZArith.ZArith.
@@ -134,10 +124,10 @@ Class IsGrpHom (A B : Type)
   (X : A -> A -> Prop) (x : A) (f : A -> A) (k : A -> A -> A)
   (Y : B -> B -> Prop) (y : B) (g : B -> B) (m : B -> B -> B)
   (h : A -> B) : Prop := {
-  dom_is_grp :> IsGrp X x f k;
-  codom_is_grp :> IsGrp Y y g m;
-  hom_is_bin_pres :> IsBinPres Y k m h;
-  hom_is_proper :> IsProper (X ==> Y) h;
+  grp_hom_dom_is_grp :> IsGrp X x f k;
+  grp_hom_codom_is_grp :> IsGrp Y y g m;
+  grp_hom_is_bin_pres :> IsBinPres Y k m h;
+  grp_hom_is_proper :> IsProper (X ==> Y) h;
 }.
 
 Section Context.
@@ -166,10 +156,9 @@ Ltac note := progress (
   try change g with (un_op (A := B)) in *;
   try change m with (bin_op (A := B)) in *).
 
-#[local] Instance hom_is_null_pres : IsNullPres Y x y h.
+#[export] Instance grp_hom_is_null_pres : IsNullPres Y x y h.
 Proof.
-  unfold IsNullPres.
-  note.
+  unfold IsNullPres. note.
   pose proof bin_pres 0 0 as a.
   setoid_rewrite <- (unl_r (h (0 + 0))) in a.
   setoid_rewrite (unl_l 0) in a.
@@ -177,10 +166,9 @@ Proof.
   setoid_rewrite <- a.
   reflexivity. Qed.
 
-#[local] Instance hom_is_un_pres : IsUnPres Y f g h.
+#[export] Instance grp_hom_is_un_pres : IsUnPres Y f g h.
 Proof.
-  note.
-  intros z.
+  note. intros z.
   pose proof bin_pres z (- z) as a.
   setoid_rewrite (inv_r z) in a.
   eapply cancel_l with (h z).
@@ -194,101 +182,9 @@ End Context.
 
 Class IsGrpActL (A B : Type)
   (X : A -> A -> Prop) (x : A) (f : A -> A) (k : A -> A -> A)
-  (Y : B -> B -> Prop) (a : A -> B -> B) : Prop := {
-  is_grp :> IsGrp X x f k;
-  act_is_unl_l :> IsUnlL Y x a;
-  act_is_assoc :> IsCompatL Y k a;
-  act_is_proper :> IsProper (X ==> Y ==> Y) a;
+  (Y : B -> B -> Prop) (al : A -> B -> B) : Prop := {
+  grp_act_l_is_grp :> IsGrp X x f k;
+  grp_act_l_is_unl_l :> IsUnlL Y x al;
+  grp_act_l_is_assoc :> IsCompatL Y k al;
+  grp_act_l_is_proper :> IsProper (X ==> Y ==> Y) al;
 }.
-
-(** Now, let us make a mess! *)
-
-From DEZ.Has Require Import
-  Decisions.
-From DEZ.Is Require Import
-  Extensional.
-From Coq Require Import
-  Extraction Lists.List ZArith.ZArith.
-
-Module Mess.
-
-(** This alternative definition is closer to the one in abstract algebra. *)
-
-Module Existential.
-
-#[local] Reserved Notation "'f'".
-
-Class IsGrp (A : Type) (X : A -> A -> Prop)
-  (x : A) (k : A -> A -> A) : Type := {
-  is_mon :> IsMon X x k;
-  inv_l_r (y : A) : {z : A | X (k z y) x /\ X (k y z) x}
-    where "'f'" := (fun x : A => proj1_sig (inv_l_r x));
-  is_proper :> IsProper (X ==> X) f;
-}.
-
-End Existential.
-
-(** The definitions are equivalent. *)
-
-Section Context.
-
-Lemma choice (A B : Type) (X : A -> B -> Prop) :
-  (forall x : A, {y : B | X x y}) -> {f : A -> B | forall x : A, X x (f x)}.
-Proof.
-  intro Hs. exists (fun x : A => proj1_sig (Hs x)).
-  intros x. destruct (Hs x) as [y HX]. cbn. apply HX. Defined.
-
-Lemma cochoice (A B : Type) (X : A -> B -> Prop) :
-  {f : A -> B | forall x : A, X x (f x)} -> forall x : A, {y : B | X x y}.
-Proof.
-  intros [f HX]. intros x. exists (f x). cbn. apply (HX x). Defined.
-
-Lemma choiceT (A B : Type) (X : A -> B -> Type) :
-  (forall x : A, {y : B & X x y}) -> {f : A -> B & forall x : A, X x (f x)}.
-Proof.
-  intro Hs. exists (fun x : A => projT1 (Hs x)).
-  intros x. destruct (Hs x) as [y HX]. cbn. apply HX. Defined.
-
-Lemma cochoiceT (A B : Type) (X : A -> B -> Type) :
-  {f : A -> B & forall x : A, X x (f x)} -> forall x : A, {y : B & X x y}.
-Proof.
-  intros [f HX]. intros x. exists (f x). cbn. apply (HX x). Defined.
-
-Lemma sectT `(!IsFunExtDep) (A B : Type) (X : A -> B -> Type)
-  (a : forall x : A, {y : B & X x y}) : cochoiceT _ (choiceT a) = a.
-Proof.
-  unfold choiceT, cochoiceT. apply fun_ext_dep. intros x.
-  destruct (a x) as [y b]. f_equal. Defined.
-
-Lemma retrT `(!IsFunExtDep) (A B : Type) (X : A -> B -> Type)
-  (a : {f : A -> B & forall x : A, X x (f x)}) : choiceT (cochoiceT _ a) = a.
-Proof.
-  unfold choiceT, cochoiceT. destruct a as [f b]. f_equal. Defined.
-
-Context (A : Type) (X : A -> A -> Prop)
-  (x : A) (k : A -> A -> A).
-
-Lemma herbrandize : {f : A -> A | IsGrp X x f k} -> Existential.IsGrp X x k.
-Proof.
-  intros [f ?]. esplit. all: shelve. Unshelve.
-  - intros y. exists (f y). split.
-    + apply inv_l.
-    + apply inv_r.
-  - typeclasses eauto.
-  - intros y z a. cbv. apply is_proper. apply a. Defined.
-
-Lemma skolemize : Existential.IsGrp X x k -> {f : A -> A | IsGrp X x f k}.
-Proof.
-  intros ?.
-  set (f (y : A) := proj1_sig (Existential.inv_l_r y)).
-  set (g (y : A) := proj2_sig (Existential.inv_l_r y)).
-  exists f. esplit.
-  - typeclasses eauto.
-  - split.
-    + intros y. destruct (g y) as [l r]. apply l.
-    + intros y. destruct (g y) as [l r]. apply r.
-  - typeclasses eauto. Defined.
-
-End Context.
-
-End Mess.
